src/Export_code.thy
@@ -3,23 +3,16 @@ imports Find_tree_stack Insert_tree_stack "~~/src/HOL/Library/Code_Target_Numera
 begin
 
 
-code_printing
-  code_module "Hack" => (OCaml)
-"module X = struct
+export_code "Code_Numeral.nat_of_integer" "Code_Numeral.int_of_integer" 
 
-type key = string
-type valuet = int
+dest_core
 
-let min_leaf_size=2
-let max_leaf_size=4
-let min_node_keys=2
-let max_node_keys=4
+mk_fts step_fts dest_fts 
+  wellformed_fts wf_fts_trans Find_tree_stack.focus_to_leaves
 
-let keyord k1 k2 = Pervasives.compare k1 k2  
+mk_its_state step_its dest_its_state  
+  wellformed_its_state wf_its_trans Insert_tree_stack.focus_to_leaves
 
-end"
-
-
-export_code "Code_Numeral.nat_of_integer" "Code_Numeral.int_of_integer" mk_fts step_fts dest_fts mk_its step_its dest_its in OCaml file "ocaml/btree_generated.ml"
+in OCaml file "ocaml/btree_generated.ml"
 
 end
